Update timing/riscvTiming.v, timing/examples/FreeRTOS_tasks_proofs.v files Deleted timing/debugging_freertos.v

timing/examples/FreeRTOS_tasks_proofs.v
@@ -2,12 +2,186 @@ Require Import lifted_RTOSDemo.
 Require Import riscvTiming.
 Import RISCVNotations.
 
+Definition vTaskSwitchContext (a : addr) : N :=
+    match a with
+    (* <vApplicationStackOverflowHook> *)
+    | 0x80012270 => 0x80014537 (* lui a0,0x80014  *)
+    | 0x80012274 => 0xff010113 (* add sp,sp,-16  *)
+    | 0x80012278 => 0x46050513 (* add a0,a0,1120 # 80014460 <_etext+0x890>  *)
+    | 0x8001227c => 0x00112623 (* sw ra,12(sp)  *)
+    (* WARNING/TODO/NOTICE : 
+        I'm manually replacing the instruction here at 0x80012280:
+            0x20d000ef (* jal 80012c8c <printf> *)
+        with a nop:
+            0x00000013 (* addi zero, zero, 0 *)
+        This is because dealing with printf is a huge pain for my timing proof,
+        and this goes into an infinite loop (by design)anyways just a few 
+        instructions later! So replacing this call has no bearing on a timing
+        proof (although it may have a bearing on future correctness proofs)
+
+        This is a lot easier than recompiling the operating system :)
+    *)
+    (* | 0x80012280 => 0x20d000ef (* jal 80012c8c <printf>  *) *)
+    | 0x80012280 => 0x00000013 (* addi zero, zero, 0 *)
+    (* TODO 
+       switch this back to
+            0x30047073 (* csrc mstatus,8  *)
+       I don't want to implement the ZICSR extension rn
+    *)
+    (* | 0x80012284 => 0x30047073 (* csrc mstatus,8  *) *)
+    | 0x80012284 => 0x00000013 (* addi zero, zero, 0 *)
+    | 0x80012288 => 0x0000006f (* j 80012288 <vApplicationStackOverflowHook+0x18>  *)
+    (* <vAssertCalled> *)
+    | 0x80012290 => 0x00050613 (* mv a2,a0  *)
+    | 0x80012294 => 0x80014537 (* lui a0,0x80014  *)
+    | 0x80012298 => 0xfe010113 (* add sp,sp,-32  *)
+    | 0x8001229c => 0x47c50513 (* add a0,a0,1148 # 8001447c <_etext+0x8ac>  *)
+    | 0x800122a0 => 0x00112e23 (* sw ra,28(sp)  *)
+    | 0x800122a4 => 0x00012623 (* sw zero,12(sp)  *)
+    (* WARNING/TODO/NOTICE : 
+        I'm manually replacing the instruction here at 0x80012280:
+            0x20d000ef (* jal 80012c8c <printf> *)
+        with a nop:
+            0x00000013 (* addi zero, zero, 0 *)
+        This is because dealing with printf is a huge pain for my timing proof,
+        and this goes into an infinite loop (by design)anyways just a few 
+        instructions later! So replacing this call has no bearing on a timing
+        proof (although it may have a bearing on future correctness proofs)
+
+        This is a lot easier than recompiling the operating system :)
+    *)
+    (* | 0x800122a8 => 0x1e5000ef (* jal 80012c8c <printf>  *) *)
+    | 0x800122a8 => 0x00000013 (* addi zero, zero, 0 *)
+    (* TODO 
+       switch this back to
+            0x30047073 (* csrc mstatus,8  *)
+       I don't want to implement the ZICSR extension rn
+    *)
+    (* | 0x800122ac => 0x30047073 (* csrc mstatus,8  *) *)
+    | 0x800122ac => 0x00000013 (* addi zero, zero, 0 *)
+    | 0x800122b0 => 0x80080737 (* lui a4,0x80080  *)
+    | 0x800122b4 => 0x00472783 (* lw a5,4(a4) # 80080004 <xCriticalNesting>  *)
+    | 0x800122b8 => 0x00178793 (* add a5,a5,1  *)
+    | 0x800122bc => 0x00f72223 (* sw a5,4(a4)  *)
+    | 0x800122c0 => 0x00c12783 (* lw a5,12(sp)  *)
+    | 0x800122c4 => 0x02078263 (* beqz a5,800122e8 <vAssertCalled+0x58>  *)
+    | 0x800122c8 => 0x00472783 (* lw a5,4(a4)  *)
+    | 0x800122cc => 0xfff78793 (* add a5,a5,-1  *)
+    | 0x800122d0 => 0x00f72223 (* sw a5,4(a4)  *)
+    | 0x800122d4 => 0x00079463 (* bnez a5,800122dc <vAssertCalled+0x4c>  *)
+    (* TODO 
+       switch this back to
+            0x30047073 (* csrc mstatus,8  *)
+       I don't want to implement the ZICSR extension rn
+    *)
+    (* | 0x800122d8 => 0x30046073 (* csrs mstatus,8  *) *)
+    | 0x800122d8 => 0x00000013 (* addi zero, zero, 0*)
+    | 0x800122dc => 0x01c12083 (* lw ra,28(sp)  *)
+    | 0x800122e0 => 0x02010113 (* add sp,sp,32  *)
+    | 0x800122e4 => 0x00008067 (* ret  *)
+    | 0x800122e8 => 0x00000013 (* nop  *)
+    | 0x800122ec => 0x00000013 (* nop  *)
+    | 0x800122f0 => 0xfd1ff06f (* j 800122c0 <vAssertCalled+0x30>  *)
+    (* <__clzsi2> *)
+    | 0x80013680 => 0x000107b7 (* lui a5,0x10  *)
+    | 0x80013684 => 0x02f57a63 (* bgeu a0,a5,800136b8 <__clzsi2+0x38>  *)
+    | 0x80013688 => 0x10053793 (* sltiu a5,a0,256  *)
+    | 0x8001368c => 0x0017b793 (* seqz a5,a5  *)
+    | 0x80013690 => 0x00379793 (* sll a5,a5,0x3  *)
+    | 0x80013694 => 0x80015737 (* lui a4,0x80015  *)
+    | 0x80013698 => 0x02000693 (* li a3,32  *)
+    | 0x8001369c => 0x40f686b3 (* sub a3,a3,a5  *)
+    | 0x800136a0 => 0x00f55533 (* srl a0,a0,a5  *)
+    | 0x800136a4 => 0xc5c70793 (* add a5,a4,-932 # 80014c5c <__clz_tab>  *)
+    | 0x800136a8 => 0x00a787b3 (* add a5,a5,a0  *)
+    | 0x800136ac => 0x0007c503 (* lbu a0,0(a5) # 10000 <__stack_size+0xfea2>  *)
+    | 0x800136b0 => 0x40a68533 (* sub a0,a3,a0  *)
+    | 0x800136b4 => 0x00008067 (* ret  *)
+    | 0x800136b8 => 0x01000737 (* lui a4,0x1000  *)
+    | 0x800136bc => 0x01800793 (* li a5,24  *)
+    | 0x800136c0 => 0xfce57ae3 (* bgeu a0,a4,80013694 <__clzsi2+0x14>  *)
+    | 0x800136c4 => 0x01000793 (* li a5,16  *)
+    | 0x800136c8 => 0xfcdff06f (* j 80013694 <__clzsi2+0x14>  *)
+    (* <vTsakSwitchContext> *)
+    | 0x800015e0 => 0x8601a703 (* lw a4,-1952(gp) # 80080060 <uxSchedulerSuspended>  *)
+    | 0x800015e4 => 0x00070863 (* beqz a4,800015f4 <vTaskSwitchContext+0x14>  *)
+    | 0x800015e8 => 0x00100713 (* li a4,1  *)
+    | 0x800015ec => 0x86e1aa23 (* sw a4,-1932(gp) # 80080074 <xYieldPendings>  *)
+    | 0x800015f0 => 0x00008067 (* ret  *)
+    | 0x800015f4 => 0xff010113 (* add sp,sp,-16  *)
+    | 0x800015f8 => 0x8601aa23 (* sw zero,-1932(gp) # 80080074 <xYieldPendings>  *)
+    | 0x800015fc => 0x01212023 (* sw s2,0(sp)  *)
+    | 0x80001600 => 0x8981a783 (* lw a5,-1896(gp) # 80080098 <pxCurrentTCB>  *)
+    | 0x80001604 => 0xa5a5a737 (* lui a4,0xa5a5a  *)
+    | 0x80001608 => 0x00112623 (* sw ra,12(sp)  *)
+    | 0x8000160c => 0x0307a783 (* lw a5,48(a5)  *)
+    | 0x80001610 => 0x00812423 (* sw s0,8(sp)  *)
+    | 0x80001614 => 0x00912223 (* sw s1,4(sp)  *)
+    | 0x80001618 => 0x0007a603 (* lw a2,0(a5)  *)
+    | 0x8000161c => 0x5a570713 (* add a4,a4,1445 # a5a5a5a5 <_stack_top+0x259c48b7>  *)
+    | 0x80001620 => 0x00e61e63 (* bne a2,a4,8000163c <vTaskSwitchContext+0x5c>  *)
+    | 0x80001624 => 0x0047a683 (* lw a3,4(a5)  *)
+    | 0x80001628 => 0x00c69a63 (* bne a3,a2,8000163c <vTaskSwitchContext+0x5c>  *)
+    | 0x8000162c => 0x0087a703 (* lw a4,8(a5)  *)
+    | 0x80001630 => 0x00d71663 (* bne a4,a3,8000163c <vTaskSwitchContext+0x5c>  *)
+    | 0x80001634 => 0x00c7a783 (* lw a5,12(a5)  *)
+    | 0x80001638 => 0x00e78a63 (* beq a5,a4,8000164c <vTaskSwitchContext+0x6c>  *)
+    | 0x8000163c => 0x8981a583 (* lw a1,-1896(gp) # 80080098 <pxCurrentTCB>  *)
+    | 0x80001640 => 0x8981a503 (* lw a0,-1896(gp) # 80080098 <pxCurrentTCB>  *)
+    | 0x80001644 => 0x03458593 (* add a1,a1,52  *)
+    | 0x80001648 => 0x429100ef (* jal 80012270 <vApplicationStackOverflowHook>  *)
+    | 0x8000164c => 0x8801a503 (* lw a0,-1920(gp) # 80080080 <uxTopReadyPriority>  *)
+    | 0x80001650 => 0x01f00493 (* li s1,31  *)
+    | 0x80001654 => 0x02c120ef (* jal 80013680 <__clzsi2>  *)
+    | 0x80001658 => 0x40a484b3 (* sub s1,s1,a0  *)
+    | 0x8000165c => 0x01400713 (* li a4,20  *)
+    | 0x80001660 => 0x02e48733 (* mul a4,s1,a4  *)
+    | 0x80001664 => 0xc6418793 (* add a5,gp,-924 # 80080464 <pxReadyTasksLists>  *)
+    | 0x80001668 => 0xc6418413 (* add s0,gp,-924 # 80080464 <pxReadyTasksLists>  *)
+    | 0x8000166c => 0x00e787b3 (* add a5,a5,a4  *)
+    | 0x80001670 => 0x0007a783 (* lw a5,0(a5)  *)
+    | 0x80001674 => 0x00079c63 (* bnez a5,8000168c <vTaskSwitchContext+0xac>  *)
+    | 0x80001678 => 0x000015b7 (* lui a1,0x1  *)
+    | 0x8000167c => 0x80014537 (* lui a0,0x80014  *)
+    | 0x80001680 => 0x41358593 (* add a1,a1,1043 # 1413 <__stack_size+0x12b5>  *)
+    | 0x80001684 => 0xbd050513 (* add a0,a0,-1072 # 80013bd0 <_etext>  *)
+    | 0x80001688 => 0x409100ef (* jal 80012290 <vAssertCalled>  *)
+    | 0x8000168c => 0x01400793 (* li a5,20  *)
+    | 0x80001690 => 0x02f487b3 (* mul a5,s1,a5  *)
+    | 0x80001694 => 0x00f40733 (* add a4,s0,a5  *)
+    | 0x80001698 => 0x00472683 (* lw a3,4(a4)  *)
+    | 0x8000169c => 0x00878793 (* add a5,a5,8  *)
+    | 0x800016a0 => 0x00f407b3 (* add a5,s0,a5  *)
+    | 0x800016a4 => 0x0046a683 (* lw a3,4(a3)  *)
+    | 0x800016a8 => 0x00d72223 (* sw a3,4(a4)  *)
+    | 0x800016ac => 0x00f69663 (* bne a3,a5,800016b8 <vTaskSwitchContext+0xd8>  *)
+    | 0x800016b0 => 0x00c72783 (* lw a5,12(a4)  *)
+    | 0x800016b4 => 0x00f72223 (* sw a5,4(a4)  *)
+    | 0x800016b8 => 0x01400793 (* li a5,20  *)
+    | 0x800016bc => 0x02f484b3 (* mul s1,s1,a5  *)
+    | 0x800016c0 => 0x00c12083 (* lw ra,12(sp)  *)
+    | 0x800016c4 => 0x00940433 (* add s0,s0,s1  *)
+    | 0x800016c8 => 0x00442783 (* lw a5,4(s0)  *)
+    | 0x800016cc => 0x00812403 (* lw s0,8(sp)  *)
+    | 0x800016d0 => 0x00412483 (* lw s1,4(sp)  *)
+    | 0x800016d4 => 0x00c7a783 (* lw a5,12(a5)  *)
+    | 0x800016d8 => 0x88f1ac23 (* sw a5,-1896(gp) # 80080098 <pxCurrentTCB>  *)
+    | 0x800016dc => 0x8981a783 (* lw a5,-1896(gp) # 80080098 <pxCurrentTCB>  *)
+    | 0x800016e0 => 0x00012903 (* lw s2,0(sp)  *)
+    | 0x800016e4 => 0x01010113 (* add sp,sp,16  *)
+    | 0x800016e8 => 0x00008067 (* ret  *)
+    | _ => 0
+    end.
+
+Definition start_vTaskSwitchContext : N := 0x800015e0.
+Definition end_vTaskSwitchContext : N := 0x800016e8.
+
 Variable ML : N.
 Variable ML_pos : 1 <= ML.
 
 Module riscv_toa.
     Definition time_of_addr (s : store) (a : addr) : N :=
-        match neorv32_cycles_upper_bound ML s (vTaskSwitchContext s a) with
+        match neorv32_cycles_upper_bound ML s (vTaskSwitchContext a) with
         | Some x => x | _ => 0 end.
 End riscv_toa.
 
@@ -23,104 +197,25 @@ Definition time_branch : N :=
     5 + (ML - 1).
 
 Definition uxSchedulerSuspended (gp : N) (mem : addr -> N) : N :=
-    mem Ⓓ[2144 + gp].
+    (* mem Ⓓ[2144 + gp]. *)
     (* This should actually be the below expression. Unclear on whether lifter
        has bug, seems like it isn't treating immediate as signed
     *)
-    (* mem Ⓓ[gp - 1952]. *)
+    mem Ⓓ[gp ⊖ 1952].
 
 Definition addr_xYieldPendings (gp : N) : N :=
     gp - 1932.
 
 Definition pxCurrentTCB (gp : N) (mem : addr -> N) : N :=
-    mem Ⓓ[2200 + gp].
+    (* mem Ⓓ[2200 + gp]. *)
     (* Same as above *)
-    (* mem Ⓓ[gp - 1896]. *)
+    mem Ⓓ[gp ⊖ 1896].
 
 Definition uxTopReadyPriority (gp : N) (mem : addr -> N) : N :=
-    mem Ⓓ[gp - 1920].
+    mem Ⓓ[gp ⊖ 1920].
 
 Definition addr_pxReadyTasksLists (gp : N) : N :=
     gp - 924.
-
-(* 
-(* <vTaskSwitchContext> *)
-    | 0x800015e0 => 0x8601a703 (* lw a4,-1952(gp) # 80080060 <uxSchedulerSuspended>  *) time_mem
-    | 0x800015e4 => 0x00070863 (* beqz a4,800015f4 <vTaskSwitchContext+0x14>  *)
-        if uxSchedulerSuspended (s R_GP) mem =? 0 then time_branch else 3
-    | 0x800015e8 => 0x00100713 (* li a4,1  *)                                           2
-    | 0x800015ec => 0x86e1aa23 (* sw a4,-1932(gp) # 80080074 <xYieldPendings>  *)       time_mem
-    | 0x800015f0 => 0x00008067 (* ret  *)                                               time_branch
-    | 0x800015f4 => 0xff010113 (* add sp,sp,-16  *)                                     2
-    | 0x800015f8 => 0x8601aa23 (* sw zero,-1932(gp) # 80080074 <xYieldPendings>  *)     time_mem
-    | 0x800015fc => 0x01212023 (* sw s2,0(sp)  *)                                       time_mem
-    | 0x80001600 => 0x8981a783 (* lw a5,-1896(gp) # 80080098 <pxCurrentTCB>  *)         time_mem
-    | 0x80001604 => 0xa5a5a737 (* lui a4,0xa5a5a  *)                                    2
-    | 0x80001608 => 0x00112623 (* sw ra,12(sp)  *)                                      time_mem
-    | 0x8000160c => 0x0307a783 (* lw a5,48(a5)  *)                                      time_mem
-    | 0x80001610 => 0x00812423 (* sw s0,8(sp)  *)                                       time_mem
-    | 0x80001614 => 0x00912223 (* sw s1,4(sp)  *)                                       time_mem
-    | 0x80001618 => 0x0007a603 (* lw a2,0(a5)  *)                                       time_mem
-    | 0x8000161c => 0x5a570713 (* add a4,a4,1445 # a5a5a5a5 <_stack_top+0x259c48b7>  *) 2
-    | 0x80001620 => 0x00e61e63 (* bne a2,a4,8000163c <vTaskSwitchContext+0x5c>  *)
-        if mem Ⓓ[mem Ⓓ[48 + pxCurrentTCB gp mem]] !=? 0xa5a5a5a5 then time_branch else 3
-    | 0x80001624 => 0x0047a683 (* lw a3,4(a5)  *)                                       time_mem
-    | 0x80001628 => 0x00c69a63 (* bne a3,a2,8000163c <vTaskSwitchContext+0x5c>  *)
-        if mem Ⓓ[4 + (48 + pxCurrentTCB gp mem)] !=? mem Ⓓ[mem Ⓓ[48 + pxCurrentTCB gp mem]] then time_branch else 3
-    | 0x8000162c => 0x0087a703 (* lw a4,8(a5)  *)                                       time_mem
-    | 0x80001630 => 0x00d71663 (* bne a4,a3,8000163c <vTaskSwitchContext+0x5c>  *)
-        if mem Ⓓ[8 + (48 + pxCurrentTCB gp mem)] !=? mem Ⓓ[4 + (48 + pxCurrentTCB gp mem)] then time_branch else 3
-    | 0x80001634 => 0x00c7a783 (* lw a5,12(a5)  *)                                      time_mem
-    | 0x80001638 => 0x00e78a63 (* beq a5,a4,8000164c <vTaskSwitchContext+0x6c>  *)
-        if mem Ⓓ[12 + (48 + pxCurrentTCB gp mem)] !=? mem Ⓓ[8 + (48 + pxCurrentTCB gp mem)] then time_branch else 3
-    | 0x8000163c => 0x8981a583 (* lw a1,-1896(gp) # 80080098 <pxCurrentTCB>  *)         time_mem
-    | 0x80001640 => 0x8981a503 (* lw a0,-1896(gp) # 80080098 <pxCurrentTCB>  *)         time_mem
-    | 0x80001644 => 0x03458593 (* add a1,a1,52  *)                                      2
-    | 0x80001648 => 0x429100ef (* jal 80012270 <vApplicationStackOverflowHook>  *)      time_branch + timeof(vApplicationStackOverflowHook)
-    | 0x8000164c => 0x8801a503 (* lw a0,-1920(gp) # 80080080 <uxTopReadyPriority>  *)   time_mem
-    | 0x80001650 => 0x01f00493 (* li s1,31  *)                                          2
-    | 0x80001654 => 0x02c120ef (* jal 80013680 <__clzsi2>  *)                           time_branch + timeof(__clzsi2)
-    | 0x80001658 => 0x40a484b3 (* sub s1,s1,a0  *)                                      2
-    | 0x8000165c => 0x01400713 (* li a4,20  *)                                          2
-    | 0x80001660 => 0x02e48733 (* mul a4,s1,a4  *)                                      2
-    | 0x80001664 => 0xc6418793 (* add a5,gp,-924 # 80080464 <pxReadyTasksLists>  *)     2
-    | 0x80001668 => 0xc6418413 (* add s0,gp,-924 # 80080464 <pxReadyTasksLists>  *)     2
-    | 0x8000166c => 0x00e787b3 (* add a5,a5,a4  *)                                      2
-    | 0x80001670 => 0x0007a783 (* lw a5,0(a5)  *)                                       time_mem
-    | 0x80001674 => 0x00079c63 (* bnez a5,8000168c <vTaskSwitchContext+0xac>  *)
-        if mem Ⓓ[(GP - 924) + ((31 - mem Ⓓ[GP - 1920]) * 20)] !=? 0 then time_branch else 3
-    | 0x80001678 => 0x000015b7 (* lui a1,0x1  *)                                        2
-    | 0x8000167c => 0x80014537 (* lui a0,0x80014  *)                                    2
-    | 0x80001680 => 0x41358593 (* add a1,a1,1043 # 1413 <__stack_size+0x12b5>  *)       2
-    | 0x80001684 => 0xbd050513 (* add a0,a0,-1072 # 80013bd0 <_etext>  *)               2
-    | 0x80001688 => 0x409100ef (* jal 80012290 <vAssertCalled>  *)                      time_branch + timeof(vAssertCalled)
-    | 0x8000168c => 0x01400793 (* li a5,20  *)                                          2
-    | 0x80001690 => 0x02f487b3 (* mul a5,s1,a5  *)                                      2
-    | 0x80001694 => 0x00f40733 (* add a4,s0,a5  *)                                      2
-    | 0x80001698 => 0x00472683 (* lw a3,4(a4)  *)                                       time_mem
-    | 0x8000169c => 0x00878793 (* add a5,a5,8  *)                                       2
-    | 0x800016a0 => 0x00f407b3 (* add a5,s0,a5  *)                                      2
-    | 0x800016a4 => 0x0046a683 (* lw a3,4(a3)  *)                                       time_mem
-    | 0x800016a8 => 0x00d72223 (* sw a3,4(a4)  *)                                       time_mem
-    | 0x800016ac => 0x00f69663 (* bne a3,a5,800016b8 <vTaskSwitchContext+0xd8>  *)
-        if mem Ⓓ[4 + mem Ⓓ[4 + (addr_pxReadyTasksLists + ((31 - uxTopReadyPriority) * 20))]] !=? 
-            (addr_pxReadyTasksLists + (((31 - uxTopReadyPriority) * 20) + 8)) then time_branch else 3
-    | 0x800016b0 => 0x00c72783 (* lw a5,12(a4)  *)                                      time_mem
-    | 0x800016b4 => 0x00f72223 (* sw a5,4(a4)  *)                                       time_mem
-    | 0x800016b8 => 0x01400793 (* li a5,20  *)                                          2
-    | 0x800016bc => 0x02f484b3 (* mul s1,s1,a5  *)                                      2
-    | 0x800016c0 => 0x00c12083 (* lw ra,12(sp)  *)                                      time_mem
-    | 0x800016c4 => 0x00940433 (* add s0,s0,s1  *)                                      2
-    | 0x800016c8 => 0x00442783 (* lw a5,4(s0)  *)                                       time_mem
-    | 0x800016cc => 0x00812403 (* lw s0,8(sp)  *)                                       time_mem
-    | 0x800016d0 => 0x00412483 (* lw s1,4(sp)  *)                                       time_mem
-    | 0x800016d4 => 0x00c7a783 (* lw a5,12(a5)  *)                                      time_mem
-    | 0x800016d8 => 0x88f1ac23 (* sw a5,-1896(gp) # 80080098 <pxCurrentTCB>  *)         time_mem
-    | 0x800016dc => 0x8981a783 (* lw a5,-1896(gp) # 80080098 <pxCurrentTCB>  *)         time_mem
-    | 0x800016e0 => 0x00012903 (* lw s2,0(sp)  *)                                       time_mem
-    | 0x800016e4 => 0x01010113 (* add sp,sp,16  *)                                      2
-    | 0x800016e8 => 0x00008067 (* ret  *)                                               5 + (ML - 1)
-*)
 
 Definition vTaskSwitchContext_exit (t:trace) :=
   match t with (Addr a,_)::_ => match a with
@@ -128,35 +223,92 @@ Definition vTaskSwitchContext_exit (t:trace) :=
   | _ => false
   end | _ => false end.
 
-Definition timing_postcondition (t : trace) (gp : N) (mem : addr -> N) : Prop :=
-    cycle_count_of_trace t = if (uxSchedulerSuspended gp mem) =? 0 then 77 else 5 + time_branch + 2 * time_mem.
-
 Notation "x !=? y" := (negb (x =? y)) (at level 70, no associativity) : N_scope.
 
+Definition timing_postcondition (t : trace) (s : store) (gp : N) (mem : addr -> N) : Prop :=
+    if (uxSchedulerSuspended gp mem) !=? 0 then 
+        cycle_count_of_trace t = 5 + time_branch + 2 * time_mem
+    else
+        cycle_count_of_trace t = 47 + 5 * time_branch + 25 * time_mem.
+
 Definition gp_sp_noverlap (gp sp : N) : Prop :=
-    ~overlap 32 gp __global_size sp vTaskSwitchContext_stack_frame_size.
+    ~overlap 32 gp __global_size (sp - vTaskSwitchContext_stack_frame_size) vTaskSwitchContext_stack_frame_size.
+
+(* Axiom printf_time : N. *)
+Axiom __clzsi2_time : N.
+Axiom vAssertCalled_time : N.
+Axiom vApplicationStackOverflowHook_time : N.
+
+Fixpoint subtrace_since_address (t : trace) (a : addr) : trace :=
+    match t with
+    | (Addr a', st) :: tl => if (a =? a') then (Addr a', st) :: nil else
+        (Addr a', st) :: subtrace_since_address tl a
+    | _ => nil
+    end.
+
+Fixpoint subtrace_before_address (t : trace) (a : addr) : trace :=
+    match t with
+    | (Addr a', st) :: tl => if (a =? a') then tl else
+        subtrace_before_address tl a
+    | _ => nil
+    end.
+
+(* The goal with the above function is to use for function timing invariants, e.g.
+        cycle_count_of_trace t' = 
+            func_time + cycle_count_of_trace (subtrace_before_address t' func_entry_addr))
+    This would be nice because then you don't have to worry about annoying arithmetic.
+    
+    Unfortunately, it seems like you'd need to put an invariant like the following
+    at the JAL instruction leading into the function:
+        cycle_count_of_trace (subtrace_before_address t' func_entry_addr)) = 
+            cycle_count_of_trace t (* where t is the whole program trace *)
+    And I'm not sure if the definition of subtrace_before_address allows for this
+    to be proven and therefore utilized.
+
+    Will have to revisit later, definitely need something like this for scaling up.
+*)
 
 Definition vTaskSwitchContext_timing_invs (_ : store) (p : addr) (base_sp : N) (t:trace) :=
 match t with (Addr a, s) :: t' => match a with
-    | 0x800015e4 => Some (
-        exists mem gp, s V_MEM32 = Ⓜmem /\ s R_GP = Ⓓgp /\ s R_SP = Ⓓbase_sp /\ s R_A4 = Ⓓ(uxSchedulerSuspended gp mem) /\ gp_sp_noverlap gp base_sp /\
-        cycle_count_of_trace t' = time_mem)
-    (* The proof expressions get big, so throw in a few intermediate invariants to constrain the goal space's size *)
-    (* | 0x80001610 => Some (exists mem gp, s V_MEM32 = Ⓜmem /\ s R_GP = Ⓓgp /\ s R_SP = Ⓓ(base_sp ⊖ 16)  /\ gp_sp_noverlap gp base_sp /\
+    (* vAssertCalled *)
+    | 0x800122e4 => Some (cycle_count_of_trace t' = 
+        vAssertCalled_time + (
+            40 + 3 * time_branch + 14 * time_mem            
+        ))
+    (* vApplicationStackOverflowHook *)
+    (* NOTE : This function intentionally goes into an infinite loop when a
+       stack overflow is detected.
+        https://github.com/FreeRTOS/FreeRTOS/blob/main/FreeRTOS/Demo/RISC-V_RV32_QEMU_VIRT_GCC/main.c#L192
+       Hamlen says control flow should never go here?
+    *)
+    | 0x80012288 => Some True
+    (* __clzsi2 *)
+    (* | 0x800136b4 => Some (cycle_count_of_trace t' =
+        __clzsi2_time + 
+            ()) *)
+    (* __clzsi2 correctness spec *)
+    (* | 0x80001658 => Some (exists mem gp,
+        s R_A2 = Ⓓ(mem Ⓓ[mem Ⓓ[48 + pxCurrentTCB gp mem]]) /\
+        s R_A3 = Ⓓ(mem Ⓓ[4 + mem Ⓓ[48 + pxCurrentTCB gp mem]]) /\
         s R_A5 = Ⓓ(mem Ⓓ[48 + pxCurrentTCB gp mem]) /\
-        s R_A4 = Ⓓ(0xa5a5a) /\
-        cycle_count_of_trace t' = 4 + 6 * time_mem + time_branch
+        s R_A0 = (* bitwidth *) Ⓓ(32 - (N.log2 (uxTopReadyPriority gp mem)))
     ) *)
+    | 0x800015e4 => Some (
+        exists mem gp, s V_MEM32 = Ⓜmem /\ s R_GP = Ⓓgp /\ s R_SP = Ⓓbase_sp 
+            /\ s R_A4 = Ⓓ(uxSchedulerSuspended gp mem) /\ gp_sp_noverlap gp base_sp /\
+        cycle_count_of_trace t' = time_mem)
     | 0x80001620 => Some (exists mem gp, s V_MEM32 = Ⓜmem /\ s R_GP = Ⓓgp /\ s R_SP = Ⓓ(base_sp ⊖ 16) /\
         s R_A5 = Ⓓ(mem Ⓓ[48 + pxCurrentTCB gp mem]) /\
         s R_A2 = Ⓓ(mem Ⓓ[mem Ⓓ[48 + pxCurrentTCB gp mem]]) /\
         s R_A4 = Ⓓ((0xa5a5a << 12) + 1445) /\
+        (uxSchedulerSuspended gp mem =? 0) = true /\
         cycle_count_of_trace t' = 6 + 9 * time_mem + time_branch)
     (* | 0x80001624 => Some (exists mem gp, s V_MEM32 = Ⓜmem /\ s R_GP = Ⓓgp /\ mem Ⓓ[mem Ⓓ[48 + pxCurrentTCB gp mem]] !=? 0xa5a5a5a5 = false) *)
     | 0x80001628 => Some (exists mem gp, s V_MEM32 = Ⓜmem /\ s R_GP = Ⓓgp /\
         s R_A2 = Ⓓ(mem Ⓓ[mem Ⓓ[48 + pxCurrentTCB gp mem]]) /\
         s R_A3 = Ⓓ(mem Ⓓ[4 + mem Ⓓ[48 + pxCurrentTCB gp mem]]) /\
         s R_A5 = Ⓓ(mem Ⓓ[48 + pxCurrentTCB gp mem]) /\
+        (uxSchedulerSuspended gp mem =? 0) = true /\
         (mem Ⓓ[ mem Ⓓ[ 48 + pxCurrentTCB gp mem ] ] !=? 0xa5a5a5a5) = false /\
         cycle_count_of_trace t' = 
             (* if (mem Ⓓ[ mem Ⓓ[ 48 + pxCurrentTCB gp mem ] ] !=? 0xa5a5a5a5) then 
@@ -169,18 +321,21 @@ match t with (Addr a, s) :: t' => match a with
         s R_A5 = Ⓓ(mem Ⓓ[48 + pxCurrentTCB gp mem]) /\
         (mem Ⓓ[ mem Ⓓ[ 48 + pxCurrentTCB gp mem ] ] !=? 0xa5a5a5a5) = false /\
         (mem Ⓓ[4 + mem Ⓓ[48 + pxCurrentTCB gp mem]] !=? mem Ⓓ[mem Ⓓ[48 + pxCurrentTCB gp mem]]) = false /\
+        (uxSchedulerSuspended gp mem =? 0) = true /\
         cycle_count_of_trace t' = 12 + 11 * time_mem + time_branch
     )
     | 0x80001638 => Some (exists mem gp, s V_MEM32 = Ⓜmem /\ s R_GP = Ⓓgp /\
+        s R_A3 = Ⓓ(mem Ⓓ[4 + mem Ⓓ[48 + pxCurrentTCB gp mem]]) /\
         s R_A4 = Ⓓ(mem Ⓓ[8 + mem Ⓓ[48 + pxCurrentTCB gp mem]]) /\
         s R_A5 = Ⓓ(mem Ⓓ[12 + mem Ⓓ[48 + pxCurrentTCB gp mem]]) /\
         (mem Ⓓ[ mem Ⓓ[ 48 + pxCurrentTCB gp mem ] ] !=? 0xa5a5a5a5) = false /\
         (mem Ⓓ[4 + mem Ⓓ[48 + pxCurrentTCB gp mem]] !=? mem Ⓓ[mem Ⓓ[48 + pxCurrentTCB gp mem]]) = false /\
         (mem Ⓓ[8 + mem Ⓓ[48 + pxCurrentTCB gp mem]] !=? mem Ⓓ[4 + mem Ⓓ[48 + pxCurrentTCB gp mem]]) = false /\
+        (uxSchedulerSuspended gp mem =? 0) = true /\
         cycle_count_of_trace t' = 15 + 12 * time_mem + time_branch
     )
-    | 0x8000163c => Some (exists mem gp, s V_MEM32 = Ⓜmem /\ s R_GP = Ⓓgp /\
-        (* s R_A5 = Ⓓ(mem Ⓓ[48 + pxCurrentTCB gp mem]) /\ *)
+    (* | 0x8000163c => Some (exists mem gp, s V_MEM32 = Ⓜmem /\ s R_GP = Ⓓgp /\
+        (uxSchedulerSuspended gp mem =? 0) = true /\
         cycle_count_of_trace t' = 6 + 9 * time_mem + time_branch + 
             (if mem Ⓓ[mem Ⓓ[ 48 + pxCurrentTCB gp mem ]] !=? 0xa5a5a5a5 then time_branch else
                 3 + 
@@ -188,36 +343,51 @@ match t with (Addr a, s) :: t' => match a with
                     time_branch + time_mem else 3 +
                     (if mem Ⓓ[8 + mem Ⓓ[48 + pxCurrentTCB gp mem]] !=? mem Ⓓ[4 + mem Ⓓ[48 + pxCurrentTCB gp mem]] then 
                         time_branch + 2 * time_mem else 3 + 3 + 3 * time_mem)))
-    )
-    | 0x80001648 => Some (exists mem gp, s V_MEM32 = Ⓜmem /\ s R_GP = Ⓓgp /\ 
+    ) *)
+     (* | 0x80001648 => Some True *)
+    (* | 0x80001648 => Some (exists mem gp, s V_MEM32 = Ⓜmem /\ s R_GP = Ⓓgp /\ 
+        (uxSchedulerSuspended gp mem =? 0) = true /\
         cycle_count_of_trace t' = 8 + 11 * time_mem + time_branch + 
             (if mem Ⓓ[mem Ⓓ[ 48 + pxCurrentTCB gp mem ]] !=? 0xa5a5a5a5 then time_branch else
                 3 + 
                 (if mem Ⓓ[4 + mem Ⓓ[48 + pxCurrentTCB gp mem]] !=? mem Ⓓ[mem Ⓓ[48 + pxCurrentTCB gp mem]] then 
                     time_branch + time_mem else 3 +
                     (if mem Ⓓ[8 + mem Ⓓ[48 + pxCurrentTCB gp mem]] !=? mem Ⓓ[4 + mem Ⓓ[48 + pxCurrentTCB gp mem]] then 
-                        time_branch + 2 * time_mem else 3 + 3 + 3 * time_mem))))
+                        time_branch + 2 * time_mem else 3 + 3 + 3 * time_mem)))) *)
     | 0x80001654 => Some (exists mem gp, s V_MEM32 = Ⓜmem /\ s R_GP = Ⓓgp /\
+        s R_S1 = Ⓓ31 /\
+        s R_A3 = Ⓓ(mem Ⓓ[4 + mem Ⓓ[48 + pxCurrentTCB gp mem]]) /\
         s R_A4 = Ⓓ(mem Ⓓ[8 + mem Ⓓ[48 + pxCurrentTCB gp mem]]) /\
         s R_A5 = Ⓓ(mem Ⓓ[12 + mem Ⓓ[48 + pxCurrentTCB gp mem]]) /\
+        (uxSchedulerSuspended gp mem =? 0) = true /\
         cycle_count_of_trace t' = 17 + 2 * time_branch + 13 * time_mem)
-    | 0x80001674 | 0x80001688 | 0x800016ac => Some (cycle_count_of_trace t' = 99)
+    | 0x80001674 => Some (exists mem gp, s V_MEM32 = Ⓜmem /\ s R_GP = Ⓓgp /\
+        s R_S0 = Ⓓ(gp ⊖ 924) /\
+        s R_A3 = Ⓓ(mem Ⓓ[4 + mem Ⓓ[48 + pxCurrentTCB gp mem]]) /\
+        s R_A4 = Ⓓ(mem Ⓓ[8 + mem Ⓓ[48 + pxCurrentTCB gp mem]]) /\
+        s R_A5 = Ⓓ(mem Ⓓ[12 + mem Ⓓ[48 + pxCurrentTCB gp mem]]) /\
+        (uxSchedulerSuspended gp mem =? 0) = true /\
+        cycle_count_of_trace t' = 29 + 2 * time_branch + 14 * time_mem)
+    | 0x80001688 => Some (exists mem gp, s V_MEM32 = Ⓜmem /\ s R_GP = Ⓓgp /\
+        s R_A3 = Ⓓ(mem Ⓓ[4 + mem Ⓓ[48 + pxCurrentTCB gp mem]]) /\
+        s R_A4 = Ⓓ(mem Ⓓ[8 + mem Ⓓ[48 + pxCurrentTCB gp mem]]) /\
+        s R_A5 = Ⓓ(mem Ⓓ[12 + mem Ⓓ[48 + pxCurrentTCB gp mem]]) /\
+        (uxSchedulerSuspended gp mem =? 0) = true /\
+        cycle_count_of_trace t' = 40 + 2 * time_branch + 14 * time_mem
+    )
+    | 0x800016ac => Some (exists mem gp, s V_MEM32 = Ⓜmem /\ s R_GP = Ⓓgp /\
+        (uxSchedulerSuspended gp mem =? 0) = true /\
+        cycle_count_of_trace t' = 39 + 3 * time_branch + 17 * time_mem
+    )
     | 0x800015f0 | 0x800016e8 => Some (
         exists mem gp, s V_MEM32 = Ⓜmem /\ s R_GP = Ⓓgp /\
-            timing_postcondition t gp mem)
+            timing_postcondition t s gp mem)
     | _ => None end
 | _ => None
 end.
 
 Definition lifted_vTaskSwitchContext : program :=
-    (* lift_via_list vTaskSwitchContext start_vTaskSwitchContext end_vTaskSwitchContext. *)
     lift_riscv vTaskSwitchContext.
-
-Compute lifted_vTaskSwitchContext empty_store start_vTaskSwitchContext.
-
-Theorem vTaskSwitchContext_welltyped: welltyped_prog rvtypctx lifted_vTaskSwitchContext.
-(* Proof. Picinae_typecheck. Qed. *)
-Admitted.
 
 Ltac unfold_decompose :=
     cbv [decompose_Btype decompose_Itype decompose_Jtype decompose_Rtype 
@@ -243,6 +413,32 @@ Ltac hammer :=
 Arguments N.add _ _ : simpl nomatch.
 Arguments N.mul _ _ : simpl nomatch.
 
+Lemma noverlap_index:
+  forall w a1 len1 a2 len2 index size
+  (NO : ~ overlap w a1 len1 a2 len2)
+  (IN : index + size <= len1),
+  ~ overlap w (a1 + index) size a2 len2.
+Proof.
+  intros.
+  remember (a1 + index) as a1'. apply noverlap_shrink with (a1:=a1) (len1:=len1).
+  rewrite Heqa1'. rewrite add_msub_l.
+  apply N.le_trans with (m:=index+size). rewrite <-N.add_le_mono_r. apply N.Div0.mod_le.
+  assumption.
+  assumption.
+Qed.
+
+Lemma getmem_nbyte_distance:
+  forall w e m a1 a2 n v,
+  msub w a1 a2 > n ->
+  msub w a2 a1 > n ->
+    getmem w e n (setmem w e n m a2 v) a1 = getmem w e n m a1.
+Proof.
+  intros.
+  apply getmem_noverlap.
+  clear - H H0.
+  apply sep_noverlap; try (left; lia || right; lia).
+Qed.
+
 Theorem vTaskSwitchContext_timing:
   forall s p t s' x' gp sp
          (ENTRY: startof t (x',s') = (Addr start_vTaskSwitchContext,s)) (* Define the entry point of the function *)
@@ -264,12 +460,14 @@ Proof using.
 
     (* Base case *)
     simpl. rewrite ENTRY. step. rename m into mem.
-    exists mem, gp. repeat split; assumption.
+    exists mem, gp. repeat split; try assumption.
+    unfold uxSchedulerSuspended. unfold msub. psimpl. reflexivity. 
 
     (* Inductive step setup *)
     intros.
     eapply startof_prefix in ENTRY; try eassumption.
-    eapply preservation_exec_prog in MDL; try eassumption; [idtac|apply vTaskSwitchContext_welltyped].
+    eapply preservation_exec_prog in MDL; 
+        try eassumption; [idtac|apply lift_riscv_welltyped].
     clear - PRE MDL. rename t1 into t. rename s1 into s'.
 
     (* Meat of proof starts here *)
@@ -279,45 +477,103 @@ Proof using.
     destruct PRE as [mem [gp [MEM [GP [SP [A4 [GP_SP_FAR Cycles]]]]]]].
     step. step. step. step. step. step. step. step. step. step. step. step.
     do 2 eexists. repeat split. unfold msub. now psimpl.
-        unfold pxCurrentTCB. admit. admit.
+        (* rewrite getmem_noverlap; cycle 1.
+            apply noverlap_shrink with (a1 := gp) (len1 := __global_size); cycle 1.
+            unfold gp_sp_noverlap in GP_SP_FAR.
+            apply noverlap_symmetry, 
+                noverlap_shrink with (a1 := (sp - vTaskSwitchContext_stack_frame_size)) (len1 := vTaskSwitchContext_stack_frame_size).
+            psimpl.  *)
+        admit. admit.
+        unfold uxSchedulerSuspended. repeat rewrite getmem_noverlap.
+            apply BC.
+        1-5: try now (apply sep_noverlap; left; unfold msub; psimpl; lia).
+        1-4: apply noverlap_shrink with (a1 := gp) (len1 := __global_size); psimpl.
+        admit. (* Overlapping stuff *)
         hammer. rewrite A4, BC, Cycles. lia.
     step. step. handle_ex.
-        unfold timing_postcondition. unfold uxSchedulerSuspended. psimpl. 
-        hammer. fold (uxSchedulerSuspended gp mem). rewrite A4, BC, Cycles. lia.
+        unfold timing_postcondition. unfold uxSchedulerSuspended in *.
+            rewrite getmem_frame; cycle 1.
+                left. psimpl. lia.
+                left. psimpl. lia.
+        rewrite BC. cbn [negb].
+        hammer. rewrite A4, BC, Cycles. lia.
     
     (* 0x80001620 *)
-    destruct PRE as [mem [gp [MEM [GP [SP [A5 [A2 [A4 Cycles]]]]]]]].
+    destruct PRE as [mem [gp [MEM [GP [SP [A5 [A2 [A4 [BR0 Cycles]]]]]]]]].
+    step.
+        step. step. step. step. step. step. step. step. step. step.
+        exact I. (* Infinite loop, stack overflow detected *)
     step. handle_ex.
         hammer. change ((678490 << 12) + 1445) with 0xa5a5a5a5 in *.
         rewrite A2, A4, BC, Cycles. lia.
-    step. handle_ex.
-        hammer. change ((678490 << 12) + 1445) with 0xa5a5a5a5 in *.
-        rewrite A2, A4, Cycles, BC. lia.
 
     (* 0x80001628 *)
-    destruct PRE as [mem [gp [MEM [GP [A2 [A3 [A5 [Br Cycles]]]]]]]].
+    destruct PRE as [mem [gp [MEM [GP [A2 [A3 [A5 [NotSuspended [Br Cycles]]]]]]]]].
     step.
-        handle_ex. hammer. change ((678490 << 12) + 1445) with 0xa5a5a5a5 in *. 
-        rewrite A2, A3, BC, Cycles, Br. lia.
-    step. handle_ex. psimpl. hammer. change ((678490 << 12) + 1445) with 0xa5a5a5a5 in *. 
+        step. step. step. step. step. step. step. step. step. step.
+        exact I. (* Infinite loop, stack overflow detected *)
+    step. handle_ex. hammer. change ((678490 << 12) + 1445) with 0xa5a5a5a5 in *. 
         rewrite A2, A3, Cycles, BC. lia.
 
     (* 0x80001630 *)
-    destruct PRE as [mem [gp [MEM [GP [A3 [A4 [A5 [B1 [B2 Cycles]]]]]]]]].
-    step. 
-        handle_ex. hammer. rewrite A3, A4, BC, B1, B2, Cycles. lia.
+    destruct PRE as [mem [gp [MEM [GP [A3 [A4 [A5 [B1 [B2 [NotSuspended Cycles]]]]]]]]]].
+    step.
+        step. step. step. step. step. step. step. step. step. step.
+        exact I. (* Infinite loop, stack overflow detected *)
     step.
         handle_ex. hammer. rewrite A3, A4, BC, Cycles. lia.
 
     (* 0x80001638 *)
-    destruct PRE as [mem [gp [MEM [GP [A4 [A5 [B1 [B2 [B3 Cycles]]]]]]]]].
-    step.
-        step. step. handle_ex. hammer. rewrite A4, A5, BC, Cycles. lia.
-    handle_ex. hammer. rewrite A4, A5, BC, Cycles, B1, B2, B3. lia.
+    destruct PRE as [mem [gp [MEM [GP [A3 [A4 [A5 [B1 [B2 [B3 [NotSuspended Cycles]]]]]]]]]]].
+    step. step. step.
+        handle_ex. hammer. rewrite A4, A5, BC, Cycles. lia.
+    step. step. step. step. step. step. step. step. step. step.
+        exact I. (* Infinite loop, stack overflow detected *)
 
-    (* 0x8000163c *)
-    destruct PRE as [mem [gp [MEM [GP Cycles]]]].
-    step. step. step. handle_ex. hammer. rewrite Cycles. psimpl. lia.
+    (* 0x80001654 *)
+    destruct PRE as [mem [gp [MEM [GP [S1 [A3 [A4 [A5 [NotSuspended Cycles]]]]]]]]].
+    admit. (* Internals of __clzsi2 *)
 
-    (* TODO : time vApplicationStackOverflowHook *)
-    step. step. (* Raise in trace here *)
+    (* 0x80001674 *)
+    destruct PRE as [mem [gp [MEM [GP [S0 [A3 [A4 [A5 [NotSuspended Cycles]]]]]]]]].
+    step. step. step. step. step. step. step. step. step.
+    handle_ex.
+        admit. (* NotSuspended overwrite goal *)
+    hammer. rewrite A5, BC, Cycles. lia.
+
+    (* 0x80001678 *)
+    step. step. step. step. 
+        handle_ex. hammer. rewrite A5, BC, Cycles. lia.
+
+    (* 0x80001688 *)
+    destruct PRE as [mem [gp [MEM [GP [A3 [A4 [A5 [NotSuspended Cycles]]]]]]]].
+    step. (* Now in vAssertCalled *)
+        admit. (* TODO : add two invariants for the branches here *)
+
+    (* 0x800016ac *)
+    destruct PRE as [mem [gp [MEM [GP [NotSuspended Cycles]]]]].
+    step. step. step. step. step. step. step. step. step.
+        step. step. step. step.
+    handle_ex. unfold timing_postcondition.
+    replace (uxSchedulerSuspended gp _ !=? 0) with false.
+    hammer. rewrite Hsv, Hsv0, BC, Cycles. lia. 
+
+    unfold "!=?". admit. (* NotSuspended overlap goal *)
+
+    (* 0x800016b0 *)
+    step. step. step. step. step. step. step. step. step.
+        step. step. step. step. step.
+    handle_ex. unfold timing_postcondition.
+    replace (uxSchedulerSuspended gp _ !=? 0) with false.
+    hammer. rewrite Hsv, Hsv0, BC, Cycles.
+    (* Need to add another set of conditions to the postcondition for this exit
+       point. Probably depends on output of __clzsi2. Where is its return value
+       stored? It seems like s1 but that don't make no sense
+    *) admit. admit. (* NotSuspended overlap goal *)
+
+    step. exact I. (* Infinite loop case *)
+
+    admit. (* Once I prove the postcondition for vAssertCalled,
+              this case should go away *)
+Admitted.
+
